Returned to multi-pass compilation

Compiler.thy
@@ -2,220 +2,8 @@ theory Compiler
   imports "02Source/AlgorithmicTypechecking" Printing "04Stack/StackConversion" 
 begin
 
-primrec get_return :: "nat \<Rightarrow> nexpr \<Rightarrow> byte_code" where
-  "get_return d (NVar x) = BReturn d"
-| "get_return d (NConst k) = BReturn d"
-| "get_return d (NLam x t e) = BReturn d"
-| "get_return d (NApp e\<^sub>1 e\<^sub>2) = BJump d"
-
-primrec compile' :: "var list \<Rightarrow> nat \<Rightarrow> nat \<Rightarrow> byte_code list \<Rightarrow> bool \<Rightarrow> nat \<Rightarrow> byte_code list \<Rightarrow> 
-    nexpr \<Rightarrow> byte_code list \<times> nat \<times> byte_code list \<times> nat" where
-  "compile' var_idxs depth sz acc tail_pos ofst lib (NVar x) = 
-    (lib, ofst, BLookup (the (idx_of var_idxs x)) # acc, Suc sz)"
-| "compile' var_idxs depth sz acc tail_pos ofst lib (NConst k) = 
-    (lib, ofst, BPushCon k # acc, Suc sz)"
-| "compile' var_idxs depth sz acc tail_pos ofst lib (NLam x t e) = (
-    let (lib', ofst', cd', sz') = compile' (x # var_idxs) (Suc depth) 0 [] True ofst lib e
-    in (lib' @ get_return (Suc depth) e # cd', 
-        Suc (ofst' + sz'),
-        BPushLam (Suc (ofst' + sz')) depth # acc,
-        Suc sz))"
-| "compile' var_idxs depth sz acc tail_pos ofst lib (NApp e\<^sub>1 e\<^sub>2) = (
-    let (lib1, ofst1, cd1, sz1) = compile' var_idxs depth sz acc False ofst lib e\<^sub>1
-    in let (lib2, ofst2, cd2, sz2) = compile' var_idxs depth sz1 cd1 False ofst1 lib1 e\<^sub>2
-    in if tail_pos then (lib2, ofst2, cd2, sz2) else (lib2, ofst2, BApply # cd2, Suc sz2))"
-
-definition compile :: "nexpr \<Rightarrow> byte_code list \<times> nat" where
-  "compile e = (  
-    let (lib, ofst, cdb, sz) = compile' [] 0 0 [] True 0 [] e
-    in (lib @ get_return 0 e # cdb, Suc (ofst + sz)))"
-
-abbreviation maybe_return :: "bool \<Rightarrow> nat" where
-  "maybe_return tail_pos \<equiv> (if tail_pos then 1 else 0)"
-
-primrec tco_code_size :: "bool \<Rightarrow> nexpr \<Rightarrow> nat" where
-  "tco_code_size tail_pos (NVar x) = 1 + maybe_return tail_pos"
-| "tco_code_size tail_pos (NConst k) = 1 + maybe_return tail_pos"
-| "tco_code_size tail_pos (NLam x t e) = 1 + tco_code_size True e + maybe_return tail_pos"
-| "tco_code_size tail_pos (NApp e\<^sub>1 e\<^sub>2) = 
-    1 + tco_code_size False e\<^sub>1 + tco_code_size False e\<^sub>2"
-
-lemma [simp]: "cd \<noteq> [] \<Longrightarrow> code_list_size (tco_cd_one op # cd) = 
-    code_size (tco_cd_one op) + code_list_size cd"
-  by (induction op) simp_all
-
-lemma [simp]: "cd' \<noteq> [] \<Longrightarrow> code_list_size (map tco_cd_one cd @ cd') = 
-  code_list_size (map tco_cd_one cd) + code_list_size cd' - 1"
-proof (induction cd)
-  case (Cons op cd)
-  thus ?case by (cases "code_list_size cd'") simp_all
-qed simp_all
-
-lemma tco_code_size_as_code_list_size [simp]: "tco_code_size True e =
-    code_list_size (tco_cd (encode' (convert' var_idxs e) depth))"
-  and [simp]: "tco_code_size False e =
-    code_list_size (map tco_cd_one (encode' (convert' var_idxs e) depth)) - 1"
-proof (induction e arbitrary: var_idxs depth)
-  case (NApp e1 e2) case 1
-  let ?cd1 = "map tco_cd_one (encode' (convert' var_idxs e1) depth)"
-  let ?cd2 = "map tco_cd_one (encode' (convert' var_idxs e2) depth)"
-  have "Suc ((code_list_size ?cd1 - 1) + (code_list_size ?cd2 - 1)) = 
-    code_list_size ?cd1 + code_list_size ?cd2 - 1" 
-      by (cases "code_list_size ?cd1") simp_all
-  with NApp show ?case by simp
-next 
-  case (NApp e1 e2) case 2
-  let ?cd1 = "map tco_cd_one (encode' (convert' var_idxs e1) depth)"
-  let ?cd2 = "map tco_cd_one (encode' (convert' var_idxs e2) depth)"
-  have "Suc ((code_list_size ?cd1 - 1) + (code_list_size ?cd2 - 1)) = 
-    code_list_size ?cd1 + code_list_size ?cd2 - 1" 
-      by (cases "code_list_size ?cd1") simp_all
-  with NApp show ?case by simp
-qed simp_all
-
-lemma compile_lengths [simp]: 
-  "compile' var_idxs depth (length acc) acc tail_pos (length lib) lib e = (lib', ofst, cd, sz) \<Longrightarrow> 
-    sz = length cd \<and> ofst = length lib'"
-proof (induction e arbitrary: var_idxs depth acc tail_pos lib lib' cd sz ofst)
-  case (NLam x t e)
-  from NLam(2) obtain lib'' ofst'' cd' sz'' where 
-    "compile' (x # var_idxs) (Suc depth) 0 [] True (length lib) lib e = (lib'', ofst'', cd', sz'') \<and>
-      lib' = lib'' @ get_return (Suc depth) e # cd' \<and> 
-        cd = BPushLam (Suc (ofst'' + sz'')) depth # acc \<and> sz = Suc (length acc) \<and> 
-          ofst = Suc (ofst'' + sz'')"
-      by (cases "compile' (x # var_idxs) (Suc depth) 0 [] True (length lib) lib e") auto
-  moreover from NLam(1) have "compile' (x # var_idxs) (Suc depth) 0 [] True (length lib) lib e = 
-    (lib'', ofst'', cd', sz'') \<Longrightarrow> sz'' = length cd' \<and> ofst'' = length lib''" 
-      by (metis list.size(3))
-  ultimately show ?case by simp
-next
-  case (NApp e1 e2)
-  obtain lib1 ofst1 cd1 sz1 where C1: 
-    "compile' var_idxs depth (length acc) acc False (length lib) lib e1 = (lib1, ofst1, cd1, sz1)" 
-      by (cases "compile' var_idxs depth (length acc) acc False (length lib) lib e1") fastforce+
-  obtain lib2 ofst2 cd2 sz2 where C2: 
-    "compile' var_idxs depth sz1 cd1 False ofst1 lib1 e2 = (lib2, ofst2, cd2, sz2)"
-      by (cases "compile' var_idxs depth sz1 cd1 False ofst1 lib1 e2") fastforce+
-  with NApp C1 have "sz2 = length cd2 \<and> ofst2 = length lib2" by blast
-  with NApp(3) C1 C2 show ?case by (auto split: if_splits)
-qed auto
-
-lemma compile_code_size [simp]: 
-  "compile' var_idxs depth (length acc) acc tail_pos (length lib) lib e = (lib', ofst, cd, sz) \<Longrightarrow> 
-    ofst + sz + maybe_return tail_pos = length lib + length acc + tco_code_size tail_pos e"
-proof (induction e arbitrary: var_idxs depth acc tail_pos lib lib' cd sz ofst)
-  case (NLam x t e)
-  obtain lib'' ofst' cd' sz' where X:
-    "compile' (x # var_idxs) (Suc depth) 0 [] True (length lib) lib e = (lib'', ofst', cd', sz')" 
-      by (cases "compile' (x # var_idxs) (Suc depth) 0 [] True (length lib) lib e") blast
-  from NLam have "\<And>xacc. 
-    compile' (x # var_idxs) (Suc depth) (length xacc) xacc True (length lib) lib e = 
-      (lib'', ofst', cd', sz') \<Longrightarrow>
-        ofst' + sz' + maybe_return True = length lib + length xacc + tco_code_size True e" by blast
-  hence "compile' (x # var_idxs) (Suc depth) (length []) [] True (length lib) lib e = 
-    (lib'', ofst', cd', sz') \<Longrightarrow>
-      ofst' + sz' + maybe_return True = length lib + length [] + tco_code_size True e" 
-    by (metis list.size(3))
-  with X have "Suc (ofst' + sz') + Suc (length acc) = 
-    Suc (length lib + length acc + tco_code_size True e)" by simp
-  with NLam X show ?case by simp
-next
-  case (NApp e1 e2)
-  obtain lib1 ofst1 cd1 sz1 where X:
-    "compile' var_idxs depth (length acc) acc False (length lib) lib e1 = (lib1, ofst1, cd1, sz1)"
-      by (cases "compile' var_idxs depth (length acc) acc False (length lib) lib e1") blast+
-  obtain lib2 ofst2 cd2 sz2 where Y:
-    "compile' var_idxs depth sz1 cd1 False ofst1 lib1 e2 = (lib2, ofst2, cd2, sz2)"
-    by (cases "compile' var_idxs depth sz1 cd1 False ofst1 lib1 e2") blast+
-  from NApp X have Z: "ofst1 + sz1 + maybe_return False = 
-    length lib + length acc + tco_code_size False e1" by blast
-  from X have L: "sz1 = length cd1 \<and> ofst1 = length lib1" by simp
-  with NApp Y have W: "ofst2 + sz2 + maybe_return False = 
-    length lib1 + length cd1 + tco_code_size False e2" by blast
-  thus ?case
-  proof (cases tail_pos)
-    case True
-    with NApp X Y Z L W show ?thesis by simp
-  next
-    case False
-    moreover with NApp X Y have "(lib2, ofst2, BApply # cd2, Suc sz2) = (lib', ofst, cd, sz)" 
-      by simp
-    moreover from Z L W have "ofst2 + sz2 = 
-      length lib + length acc + tco_code_size False e1 + tco_code_size False e2" by simp
-    ultimately show ?thesis by fastforce
-  qed
-qed auto
-
-lemma compile_code [simp]: "compile' var_idxs depth (length acc) acc True (length lib) lib e =
-  (lib', ofst', cd', sz') \<Longrightarrow> lib' @ get_return depth e # cd' = 
-    lib @ flatten_code' (length lib) (tco_cd (encode' (convert' var_idxs e) depth)) 
-      (tco_r depth (encode' (convert' var_idxs e) depth)) @ acc"
-  and "compile' var_idxs depth (length acc) acc False (length lib) lib e =
-    (lib', ofst', cd', sz') \<Longrightarrow> undefined"
-proof (induction e arbitrary: var_idxs depth acc lib lib' ofst' cd' sz')
-  case (NVar x) case 2
-  thus ?case by simp
-next
-  case (NConst k) case 2
-  thus ?case by simp
-next
-  case (NLam x t e) case 2
-  thus ?case by simp
-next
-  case (NApp e1 e2) case 2
-  thus ?case by simp
-next
-  case (NLam x t e) case 1
-  let ?cde = "encode' (convert' (x # var_idxs) e) (Suc depth)"
-  from 1 obtain lib'' ofst'' cd'' sz'' where C: 
-    "compile' (x # var_idxs) (Suc depth) 0 [] True (length lib) lib e = 
-      (lib'', ofst'', cd'', sz'') \<and> lib' = lib'' @ get_return (Suc depth) e # cd'' \<and> 
-        cd' = BPushLam (Suc (ofst'' + sz'')) depth # acc \<and> sz' = Suc (length acc) \<and> 
-          ofst' = Suc (ofst'' + sz'')"
-    by (cases "compile' (x # var_idxs) (Suc depth) 0 [] True (length lib) lib e") auto
-  with NLam(1) have L: "lib' =
-    lib @ flatten_code' (length lib) (tco_cd ?cde) (tco_r (Suc depth) ?cde) @ []" 
-      by (metis list.size(3))
-  from C have S: "sz'' = length cd'' \<and> ofst'' = length lib''" 
-    by (metis compile_lengths list.size(3))
-  have "\<And>xacc. compile' (x # var_idxs) (Suc depth) (length xacc) xacc True (length lib) lib e = 
-    (lib'', ofst'', cd'', sz'') \<Longrightarrow> 
-      ofst'' + sz'' + maybe_return True = length lib + length xacc + tco_code_size True e"
-        using compile_code_size by blast
-  hence "compile' (x # var_idxs) (Suc depth) (length []) [] True (length lib) lib e = 
-    (lib'', ofst'', cd'', sz'') \<Longrightarrow> 
-      ofst'' + sz'' + maybe_return True = length lib + length [] + tco_code_size True e"
-        by (metis list.size(3))
-  with C S have X: "Suc (length lib'' + length cd'') = length lib + tco_code_size True e" by simp
-  have "code_list_size (tco_cd ?cde) = tco_code_size True e" 
-    by (metis tco_code_size_as_code_list_size)
-  with C L S X show ?case by (cases var_idxs) simp_all
-next
-  case (NApp e1 e2) case 1
-  obtain lib1 ofst1 cd1 sz1 where X:
-    "compile' var_idxs depth (length acc) acc False (length lib) lib e1 = (lib1, ofst1, cd1, sz1)"
-      by (cases "compile' var_idxs depth (length acc) acc False (length lib) lib e1") blast+
-  with 1 have Y: "compile' var_idxs depth sz1 cd1 False ofst1 lib1 e2 = (lib', ofst', cd', sz')"
-    by (cases "compile' var_idxs depth sz1 cd1 False ofst1 lib1 e2") simp_all
-
-
-  from NApp X have "lib1 @ get_return depth e1 # cd1 = 
-    lib @ flatten_code' (length lib) (tco_cd (encode' (convert' var_idxs e1) depth)) 
-      (tco_r depth (encode' (convert' var_idxs e1) depth)) @ acc" by simp
-
-
-  from X have "sz1 = length cd1 \<and> ofst1 = length lib1" by simp 
-  with NApp Y have "lib' @ get_return depth e2 # cd' = 
-    lib1 @ flatten_code' (length lib1) (tco_cd (encode' (convert' var_idxs e2) depth)) 
-      (tco_r depth (encode' (convert' var_idxs e2) depth)) @ cd1" by simp
-
-
-
-  have "lib' @ BJump depth # cd' =
-    lib @ flatten_code' (length lib) (map tco_cd_one (encode' (convert' var_idxs e1) depth) @ 
-      map tco_cd_one (encode' (convert' var_idxs e2) depth)) (TCOJump depth) @ acc" by simp
-  thus ?case by simp
-qed simp_all
+abbreviation compile :: "nexpr \<Rightarrow> byte_code list" where 
+  "compile \<equiv> flatten_code \<circ> tco \<circ> encode \<circ> convert"
 
 lemma [simp]: "live_frame (env, tco_cd (encode' e i), tco_r d (encode' e j))"
   by (induction e) simp_all
@@ -223,38 +11,9 @@ lemma [simp]: "live_frame (env, tco_cd (encode' e i), tco_r d (encode' e j))"
 lemma [simp]: "live_frame (env, tco_cd (encode e), tco_r d (encode e))"
   by (simp add: encode_def)
 
-lemma compile_correct: "compile e = (cd, pc) \<Longrightarrow> 
-  cd = flatten_code (tco (encode (convert e))) \<and> pc = length cd"
-proof (unfold compile_def convert_def encode_def tco_def)
-  obtain lib ofst cdb sz where C: "compile' [] 0 0 [] True 0 [] e = (lib, ofst, cdb, sz)"
-    by (cases "compile' [] 0 0 [] True 0 [] e") blast+
-  moreover assume "(let (lib, ofst, cdb, sz) = compile' [] 0 0 [] True 0 [] e
-    in (lib @ get_return 0 e # cdb, Suc (ofst + sz))) = (cd, pc)"
-  ultimately have X: "cd = lib @ get_return 0 e # cdb \<and> pc = Suc (ofst + sz)" by simp
-  have "\<And>acc xlib. compile' [] 0 (length acc) acc True (length xlib) xlib e = 
-    (lib, ofst, cdb, sz) \<Longrightarrow> lib @ get_return 0 e # cdb = 
-      xlib @ flatten_code' (length xlib) (tco_cd (encode' (convert' [] e) 0)) 
-        (tco_r 0 (encode' (convert' [] e) 0)) @ acc" by (metis compile_code)
-  hence "compile' [] 0 (length []) [] True (length []) [] e = (lib, ofst, cdb, sz) \<Longrightarrow> 
-    lib @ get_return 0 e # cdb = [] @ flatten_code' (length []) (tco_cd (encode' (convert' [] e) 0)) 
-      (tco_r 0 (encode' (convert' [] e) 0)) @ []" by (metis list.size(3))
-  with C have Y: "lib @ get_return 0 e # cdb = flatten_code' 0 (tco_cd (encode' (convert' [] e) 0)) 
-    (tco_r 0 (encode' (convert' [] e) 0))" by simp
-  have "\<And>acc xlib. compile' [] 0 (length acc) acc True (length xlib) xlib e = 
-    (lib, ofst, cdb, sz) \<Longrightarrow> 
-      ofst + sz + maybe_return True = length xlib + length acc + tco_code_size True e" 
-        using compile_code_size by blast
-  hence "compile' [] 0 (length []) [] True (length []) [] e = (lib, ofst, cdb, sz) \<Longrightarrow> 
-    ofst + sz + maybe_return True = length [] + length [] + tco_code_size True e" 
-      by (metis list.size(3))
-  with C X Y show "cd = 
-    flatten_code (tco_cd (encode' (convert' [] e) 0), tco_r 0 (encode' (convert' [] e) 0)) \<and> 
-      pc = length cd" by simp
-qed
-
-theorem tc_terminationn: "typechecks e \<Longrightarrow> compile e = (cd, pc) \<Longrightarrow> 
+theorem tc_terminationn: "typechecks e \<Longrightarrow> compile e = cd \<Longrightarrow> 
   \<exists>v. valn v \<and> e \<Down> v \<and> 
-    (\<exists>h v\<^sub>f. iter (\<leadsto>\<^sub>f) (FS hempty [] [[pc]] cd) (FS h [v\<^sub>f] [] cd) \<and> 
+    (\<exists>h v\<^sub>f. iter (\<leadsto>\<^sub>f) (FS hempty [] [[length cd]] cd) (FS h [v\<^sub>f] [] cd) \<and> 
       print_hclosure (get_closure h v\<^sub>f) = print_nexpr v)"
 proof -
   assume "typechecks e"
@@ -280,29 +39,27 @@ proof -
     (tco_state (TS [encode_closure c] []))" by (metis iter_tco_eval)
   hence ET: "iter (\<leadsto>\<^sub>t\<^sub>c\<^sub>o) (TCOS [] [([], tco_cd (encode (convert e)), tco_r 0 (encode (convert e)))]) 
     (TCOS [tco_val (encode_closure c)] [])" by simp
-  assume "compile e = (cd, pc)"
-  hence C: "cd = flatten_code (tco (encode (convert e))) \<and> pc = length cd" 
-    by (metis compile_correct)
-  hence UB: "unflatten_state (BS [] [([], pc)] cd) = 
+  assume C: "compile e = cd"
+  hence UB: "unflatten_state (BS [] [([], length cd)] cd) = 
     TCOS [] [([], tco_cd (encode (convert e)), tco_r 0 (encode (convert e)))]" 
       by (auto simp add: tco_def simp del: flatten_code.simps)
-  from C have "orderly_state (BS [] [([], pc)] cd)" by auto
+  from C have "orderly_state (BS [] [([], length cd)] cd)" by auto
   with ET UB obtain v\<^sub>b where EB: 
-    "iter (\<leadsto>\<^sub>b) (BS [] [([], pc)] cd) (BS [v\<^sub>b] [] cd) \<and> 
+    "iter (\<leadsto>\<^sub>b) (BS [] [([], length cd)] cd) (BS [v\<^sub>b] [] cd) \<and> 
       tco_val (encode_closure c) = unflatten_closure cd v\<^sub>b" 
     by (metis evalb_end byte_code_state.sel(3))
   hence "print_bclosure v\<^sub>b = print_tco_closure (tco_val (encode_closure c))" by simp
   with VC have VB: "print_bclosure v\<^sub>b = print_nexpr v\<^sub>n" by simp
-  from EB obtain \<Sigma>\<^sub>h' where EH: "iter (\<leadsto>\<^sub>h) (HS hempty [] [([], pc)] cd) \<Sigma>\<^sub>h' \<and> 
+  from EB obtain \<Sigma>\<^sub>h' where EH: "iter (\<leadsto>\<^sub>h) (HS hempty [] [([], length cd)] cd) \<Sigma>\<^sub>h' \<and> 
     BS [v\<^sub>b] [] cd = unheap \<Sigma>\<^sub>h'" by fastforce
   then obtain h\<^sub>h v\<^sub>h where SH: "\<Sigma>\<^sub>h' = HS h\<^sub>h [v\<^sub>h] [] cd \<and> v\<^sub>b = unheap_closure h\<^sub>h v\<^sub>h" 
     using unheap_empty by blast
   with VB have VH: "print_hclosure (hlookup h\<^sub>h v\<^sub>h) = print_nexpr v\<^sub>n" by simp
-  have HS: "heap_structured (HS hempty [] [([], pc)] cd)" by simp
-  have FS: "flatten (HS hempty [] [([], pc)] cd) = FS hempty [] [[pc]] cd" by simp
+  have HS: "heap_structured (HS hempty [] [([], length cd)] cd)" by simp
+  have FS: "flatten (HS hempty [] [([], length cd)] cd) = FS hempty [] [[length cd]] cd" by simp
   obtain h\<^sub>f mp where HC: "hsplay splay_closure h\<^sub>h = (h\<^sub>f, mp)" by fastforce
   with SH have "flatten \<Sigma>\<^sub>h' = FS h\<^sub>f [mp v\<^sub>h] [] cd" by simp
-  with EH FS HS have EF: "iter (\<leadsto>\<^sub>f) (FS hempty [] [[pc]] cd) (FS h\<^sub>f [mp v\<^sub>h] [] cd)"
+  with EH FS HS have EF: "iter (\<leadsto>\<^sub>f) (FS hempty [] [[length cd]] cd) (FS h\<^sub>f [mp v\<^sub>h] [] cd)"
     by (metis completef_iter)
   from EH have "heap_structured \<Sigma>\<^sub>h'" by fastforce
   with SH have "hcontains h\<^sub>h v\<^sub>h" by simp
@@ -313,7 +70,7 @@ proof -
 
 
 
-  from EF VF have "iter (\<leadsto>\<^sub>f) (FS hempty [] [[pc]] cd) (FS h\<^sub>f [mp v\<^sub>h] [] cd) \<and> 
+  from EF VF have "iter (\<leadsto>\<^sub>f) (FS hempty [] [[length cd]] cd) (FS h\<^sub>f [mp v\<^sub>h] [] cd) \<and> 
     print_hclosure (get_closure h\<^sub>f (mp v\<^sub>h)) = print_nexpr v\<^sub>n" by simp
   with EN VN show ?thesis by fastforce
 qed
